Move examples, change name

LocalLang/Typing.lean
@@ -5,35 +5,17 @@ import LocalLang.Types
 
 mutual
   inductive TypeJdg : TypeContext → Expr → LLType → Prop where
-    | JdgVar {Γ : TypeContext}  {name : String} (H : (name, LLType.nat) ∈ Γ)
+    | jdgVar {Γ : TypeContext}  {name : String} (H : (name, LLType.nat) ∈ Γ)
                       : TypeJdg Γ (.var name) LLType.nat
-    | JdgConst {Γ : TypeContext} {n : ℕ} : TypeJdg Γ (.const n) LLType.nat
-    | JdgFun {Γ : TypeContext} {es : List Expr} {arg_types : List LLType} {T_return : LLType}
+    | jdgConst {Γ : TypeContext} {n : ℕ} : TypeJdg Γ (.const n) LLType.nat
+    | jdgFun {Γ : TypeContext} {es : List Expr} {arg_types : List LLType} {T_return : LLType}
                   (H_f : (f, .func arg_types T_return) ∈ Γ)
                   (H_args : TypeJdgList Γ es arg_types)
                         : TypeJdg Γ (.funCall f es) (LLType.func arg_types T_return)
 
   inductive TypeJdgList : TypeContext -> List Expr -> List LLType -> Prop
-    | Nil : TypeJdgList Γ [] []
-    | Cons {e : Expr} {T : LLType} {es : List Expr} {Ts : List LLType}
+    | nil : TypeJdgList Γ [] []
+    | cons {e : Expr} {T : LLType} {es : List Expr} {Ts : List LLType}
           (h_e : TypeJdg Γ e T) (h_es : TypeJdgList Γ es Ts)
           : TypeJdgList Γ (e :: es) (T :: Ts)
 end
-
-
--- Examples for TypeJdg
-example : TypeJdg [] (.const 5) .nat := by
-  apply TypeJdg.JdgConst
-
-example : TypeJdg [("x", .nat)] (.var "x") .nat := by
-  apply TypeJdg.JdgVar (List.mem_singleton_self ("x", LLType.nat))
-
-def ctx : TypeContext := [("add", .func [.nat] .nat), ("x", .nat)]
-
-example : TypeJdg ctx (.funCall "add" [.var "x"]) (LLType.func [.nat] .nat) := by
-  apply TypeJdg.JdgFun (by simp [ctx]) (by
-    apply TypeJdgList.Cons
-    · apply TypeJdg.JdgVar
-      simp [ctx]
-    · apply TypeJdgList.Nil
-  )
