LocalLang/TypingExamples.lean
@@ -1,0 +1,18 @@
+import LocalLang.Typing
+
+-- Examples for TypeJdg
+example : TypeJdg [] (.const 5) .nat := by
+  apply TypeJdg.jdgConst
+
+example : TypeJdg [("x", .nat)] (.var "x") .nat := by
+  apply TypeJdg.jdgVar (List.mem_singleton_self ("x", LLType.nat))
+
+def ctx : TypeContext := [("add", .func [.nat] .nat), ("x", .nat)]
+
+example : TypeJdg ctx (.funCall "add" [.var "x"]) (LLType.func [.nat] .nat) := by
+  apply TypeJdg.jdgFun (by simp [ctx]) (by
+    apply TypeJdgList.cons
+    · apply TypeJdg.jdgVar
+      simp [ctx]
+    · apply TypeJdgList.nil
+  )
